Contexts.thy
@@ -33,27 +33,34 @@ definition subsumes :: "transition \<Rightarrow> registers \<Rightarrow> transit
                                   (\<forall>P r'. (p1 $ r' = None) \<or> (P (p2 $ r') \<longrightarrow> P (p1 $ r'))))
                       )"
 
-lemma subsumption: "(Label t1 = Label t2 \<and> Arity t1 = Arity t2) \<Longrightarrow>
+lemma subsumption:
+  "(Label t1 = Label t2 \<and> Arity t1 = Arity t2) \<Longrightarrow>
    (\<forall>i. can_take_transition t1 i r \<longrightarrow> can_take_transition t2 i r) \<Longrightarrow>
    (\<forall>i. can_take_transition t1 i r \<longrightarrow>
         apply_outputs (Outputs t1) (join_ir i r) = apply_outputs (Outputs t2) (join_ir i r)) \<Longrightarrow>
+
    (\<forall>p1 p2 i. posterior_separate (Arity t1) (Guards t1) (Updates t2) i r = Some p2 \<longrightarrow>
               posterior_separate (Arity t1) (Guards t1) (Updates t1) i r = Some p1 \<longrightarrow>
               (\<forall>P r'. (p1 $ r' = None) \<or> (P (p2 $ r') \<longrightarrow> P (p1 $ r')))) \<Longrightarrow>
    subsumes t2 r t1"
   by (simp add: subsumes_def)
 
-lemma bad_guards: "\<exists>i. can_take_transition t1 i r \<and> \<not> can_take_transition t2 i r \<Longrightarrow>
+lemma bad_guards:
+  "\<exists>i. can_take_transition t1 i r \<and> \<not> can_take_transition t2 i r \<Longrightarrow>
    \<not> subsumes t2 r t1"
   by (simp add: subsumes_def)
 
-lemma inconsistent_updates: "\<exists>p2 p1. (\<exists>i. posterior_separate (Arity t1) (Guards t1) (Updates t2) i r = Some p2 \<and>
+lemma inconsistent_updates:
+  "\<exists>p2 p1. (\<exists>i. posterior_separate (Arity t1) (Guards t1) (Updates t2) i r = Some p2 \<and>
                 posterior_separate (Arity t1) (Guards t1) (Updates t1) i r = Some p1) \<and>
            (\<exists>r' P. P (p2 $ r') \<and> (\<exists>y. p1 $ r' = Some y) \<and> \<not> P (p1 $ r')) \<Longrightarrow>
+
     \<not> subsumes t2 r t1"
   by (metis (no_types, hide_lams) option.simps(3) subsumes_def)
 
-lemma bad_outputs: "\<exists>i. can_take_transition t1 i r \<and> apply_outputs (Outputs t1) (join_ir i r) \<noteq> apply_outputs (Outputs t2) (join_ir i r) \<Longrightarrow>
+lemma bad_outputs:
+  "\<exists>i. can_take_transition t1 i r \<and> apply_outputs (Outputs t1) (join_ir i r) \<noteq> apply_outputs (Outputs t2) (join_ir i r) \<Longrightarrow>
+
  \<not> subsumes t2 r t1"
   by (simp add: subsumes_def)
 
@@ -88,11 +95,14 @@ abbreviation anterior_context :: "transition_matrix \<Rightarrow> trace \<Righta
 lemma anterior_context_empty: "anterior_context e [] = Some <>"
   by (simp add: posterior_sequence_def)
 
-lemma posterior_sequence_implies_accepting_sequence: "posterior_sequence e s d t = Some ca \<Longrightarrow> accepting_sequence e s d t [] \<noteq> None"
+lemma posterior_sequence_implies_accepting_sequence:
+  "posterior_sequence e s d t = Some ca \<Longrightarrow>
+   accepting_sequence e s d t [] \<noteq> None"
   apply (simp add: posterior_sequence_def)
   by (cases "accepting_sequence e s d t []", auto)
 
-lemma accepting_sequence_accepts: "accepting_sequence e s r t [] = Some y \<Longrightarrow> accepts e s r t"
+lemma accepting_sequence_accepts:
+  "accepting_sequence e s r t [] = Some y \<Longrightarrow> accepts e s r t"
 proof(induct t arbitrary: r)
   case Nil
   then show ?case
@@ -108,7 +118,8 @@ next
     using accepts.step random_member_Some by fastforce
 qed
 
-lemma posterior_sequence_accepts: "posterior_sequence e s d t = Some ca \<longrightarrow> accepts e s d t"
+lemma posterior_sequence_accepts:
+  "posterior_sequence e s d t = Some ca \<longrightarrow> accepts e s d t"
   using posterior_sequence_implies_accepting_sequence[of e s d t ca]
   apply simp
   apply clarify
@@ -116,13 +127,16 @@ lemma posterior_sequence_accepts: "posterior_sequence e s d t = Some ca \<longri
   using accepting_sequence_accepts
   by auto
 
-lemma anterior_context_accepts: "\<exists>c. anterior_context e p = Some c \<Longrightarrow> accepts_trace e p"
+lemma anterior_context_accepts:
+  "\<exists>c. anterior_context e p = Some c \<Longrightarrow> accepts_trace e p"
   using posterior_sequence_accepts by blast
 
-lemma posterior_sequence_gives_accept: "posterior_sequence e s d t \<noteq> None \<Longrightarrow> accepts e s d t"
+lemma posterior_sequence_gives_accept:
+  "posterior_sequence e s d t \<noteq> None \<Longrightarrow> accepts e s d t"
   using option.discI posterior_sequence_accepts by auto
 
-lemma accepting_sequence_posterior_sequence_not_none: "accepting_sequence e s d t [] \<noteq> None \<Longrightarrow>
+lemma accepting_sequence_posterior_sequence_not_none:
+  "accepting_sequence e s d t [] \<noteq> None \<Longrightarrow>
    posterior_sequence e s d t \<noteq> None"
   apply (simp add: posterior_sequence_def)
   apply (case_tac "accepting_sequence e s d t []")
@@ -131,12 +145,14 @@ lemma accepting_sequence_posterior_sequence_not_none: "accepting_sequence e s d 
   apply (case_tac "last a")
   by simp
 
-lemma posterior_sequence_none_accepting_sequence_none: "(posterior_sequence e s d t = None) = (accepting_sequence e s d t [] = None)"
+lemma posterior_sequence_none_accepting_sequence_none:
+  "(posterior_sequence e s d t = None) = (accepting_sequence e s d t [] = None)"
   apply standard
   using accepting_sequence_posterior_sequence_not_none apply blast
   by (simp add: posterior_sequence_def)
 
-lemma rejects_gives_no_accepting_sequence: "rejects e s r t \<Longrightarrow> accepting_sequence e s r t [] = None"
+lemma rejects_gives_no_accepting_sequence:
+  "rejects e s r t \<Longrightarrow> accepting_sequence e s r t [] = None"
 proof(induct t arbitrary: s r)
   case Nil
   then show ?case
@@ -152,10 +168,12 @@ next
     using accepts.step random_member_Some by fastforce
 qed
 
-lemma rejects_gives_no_posterior_sequence: "rejects e s d t \<Longrightarrow> posterior_sequence e s d t = None"
+lemma rejects_gives_no_posterior_sequence:
+  "rejects e s d t \<Longrightarrow> posterior_sequence e s d t = None"
   using posterior_sequence_gives_accept by blast
 
-lemma no_accepting_sequence_rejected: "accepting_sequence e s d t seq = None \<longrightarrow> rejects e s d t"
+lemma no_accepting_sequence_rejected:
+  "accepting_sequence e s d t seq = None \<longrightarrow> rejects e s d t"
 proof(induct t arbitrary: s d seq)
   case Nil
   then show ?case
@@ -184,18 +202,22 @@ next
     by (metis (mono_tags, lifting) case_prodD ffmember_filter random_member_Some)
 qed
 
-lemma no_posterior_sequence_reject: "posterior_sequence e s d t = None \<Longrightarrow> \<not>accepts e s d t"
+lemma no_posterior_sequence_reject:
+  "posterior_sequence e s d t = None \<Longrightarrow> \<not>accepts e s d t"
   apply (simp add: posterior_sequence_none_accepting_sequence_none)
   using no_accepting_sequence_rejected
   by blast
 
-lemma accepts_gives_context: "\<forall>s d. accepts e s d t \<longrightarrow> (\<exists>c. posterior_sequence e s d t = Some c)"
+lemma accepts_gives_context:
+  "\<forall>s d. accepts e s d t \<longrightarrow> (\<exists>c. posterior_sequence e s d t = Some c)"
   using no_posterior_sequence_reject by blast
 
-lemma accepts_trace_gives_context: "accepts_trace e p \<Longrightarrow> (\<exists>c. anterior_context e p = Some c)"
+lemma accepts_trace_gives_context:
+  "accepts_trace e p \<Longrightarrow> (\<exists>c. anterior_context e p = Some c)"
   using accepts_gives_context by auto
 
-lemma accepts_trace_anterior_not_none: "accepts_trace e p \<Longrightarrow> anterior_context e p \<noteq> None"
+lemma accepts_trace_anterior_not_none:
+  "accepts_trace e p \<Longrightarrow> anterior_context e p \<noteq> None"
   using accepts_trace_gives_context by blast
 
 lemma no_choice_no_subsumption: "Label t = Label t' \<Longrightarrow>
@@ -216,7 +238,8 @@ lemma subsumption_def_alt: "subsumes t1 c t2 = (Label t2 = Label t1 \<and>
   apply (simp add: subsumes_def posterior_separate_def can_take_transition_def[symmetric])
   by blast
 
-lemma subsumes_update_equality: "subsumes t1 c t2 \<Longrightarrow> (\<forall>i. can_take_transition t2 i c \<longrightarrow>
+lemma subsumes_update_equality:
+  "subsumes t1 c t2 \<Longrightarrow> (\<forall>i. can_take_transition t2 i c \<longrightarrow>
          (\<forall>r'.
              ((apply_updates (Updates t1) (join_ir i c) c $ r') = (apply_updates (Updates t2) (join_ir i c) c $ r')) \<or>
              apply_updates (Updates t2) (join_ir i c) c $ r' = None))"
